thy/generated/CakeML/AstAuxiliary.thy
@@ -6,6 +6,7 @@ imports
   Main
   "HOL-Library.Datatype_Records"
   "LEM.Lem_pervasives"
+  "LEM.Lem_pervasives_extra"
   "Lib"
   "Namespace"
   "FpSem"
