thy/generated/CakeML/LibAuxiliary.thy
@@ -6,8 +6,6 @@ imports
   Main
   "HOL-Library.Datatype_Records"
   "LEM.Lem_pervasives"
-  "LEM.Lem_list_extra"
-  "LEM.Lem_string"
   "Coinductive.Coinductive_List"
   "Lib"
 
